\subsubsection{Proof of the equation}
\label{sec:EquationProofNotInZK} 
What we want is to check the following equality : $(\sum_{i=0}^m a_i A_i(s)) (\sum_{i=0}^m a_i B_i(s)) = \sum_{i=0}^m a_i C_i(s) + H(s) Z(s)$
\\Detailled calculation for the if statement in verify function :
\\ UV = $(\alpha + \sum_{i=0}^{m} a_i A_i (s) + r\delta ) (\beta + \sum_{i=0}^{m} a_i B_i (s) + k\delta )$
\\
\\ = $\alpha\beta + \alpha(\sum_{i=0}^{m} a_i B_i (s)) + k\alpha\delta + \beta(\sum_{i=0}^{m} a_i A_i (s))+ (\sum_{i=0}^{m} a_i A_i (s))(\sum_{i=0}^{m} a_i B_i (s)) + k\delta(\sum_{i=0}^{m} a_i A_i (s)) + r\delta\beta + r\delta(\sum_{i=0}^{m} a_i B_i (s)+ rk\delta\delta$
\\
\\
\\ $\alpha \beta + Y \gamma +  W\delta$ = $\alpha \beta + (\frac{\beta \sum_{i=0}^{l} a_i A_i (s) + \alpha \sum_{i=0}^{l} a_i B_i(s) + \sum_{i=0}^{l} a_i C_i(s) }{\gamma}) \gamma  + (S + \frac{H(s)Z(s)}{\delta} + Uk + rV - rk\delta) \delta$
\\
\\ = $\alpha \beta + \beta \sum_{i=0}^{l} a_i A_i (s) + \alpha \sum_{i=0}^{l} a_i B_i(s) + \sum_{i=0}^{l} a_i C_i(s)  + (S + Uk + rV - rk\delta) \delta + H(s)Z(s)$
\\
\\ = $\alpha \beta + \beta \sum_{i=0}^{l} a_i A_i (s) + \alpha \sum_{i=0}^{l} a_i B_i(s) + \sum_{i=0}^{l} a_i C_i(s)  + (\frac{\beta \sum_{i=l+1}^m a_i A_i(s) + \alpha \sum_{i=l+1}^m a_i B_i(s) + \sum_{i=l+1}^m a_i C_i(s)}{\delta} + (\alpha + \sum_{i=0}^{m} a_i A_i (s) + r\delta)k + r(\beta + \sum_{i=0}^{m} a_i B_i (s) + k\delta) - rk\delta) \delta + H(s)Z(s)$
\\
\\ = $\alpha \beta + \beta \sum_{i=0}^{l} a_i A_i (s) + \alpha \sum_{i=0}^{l} a_i B_i(s) + \sum_{i=0}^{l} a_i C_i(s)  + \beta \sum_{i=l+1}^m a_i A_i(s) + \alpha \sum_{i=l+1}^m a_i B_i(s) + \sum_{i=l+1}^m a_i C_i(s) + ((\alpha + \sum_{i=0}^{m} a_i A_i (s) + r\delta)k + r(\beta + \sum_{i=0}^{m} a_i B_i (s) + k\delta) - rk\delta) \delta + H(s)Z(s)$
\\
\\ = $\alpha \beta + \beta \sum_{i=0}^{m} a_i A_i (s) + \alpha \sum_{i=0}^{m} a_i B_i(s) + \sum_{i=0}^{m} a_i C_i(s) + ((\alpha + \sum_{i=0}^{m} a_i A_i (s) + r\delta)k + r(\beta + \sum_{i=0}^{m} a_i B_i (s) + k\delta) - rk\delta) \delta + H(s)Z(s)$
\\
\\ = $\alpha \beta + \beta \sum_{i=0}^{m} a_i A_i (s) + \alpha \sum_{i=0}^{m} a_i B_i(s) + \sum_{i=0}^{m} a_i C_i(s) + (k \alpha + k \sum_{i=0}^{m} a_i A_i (s) + k r\delta + r \beta + r \sum_{i=0}^{m} a_i B_i (s) + r k\delta - rk\delta) \delta + H(s)Z(s)$
\\
\\ = $\alpha\beta + \beta\sum_{i=0}^{m} a_i A_i (s) + \alpha\sum_{i=0}^{m} a_i B_i(s) + \sum_{i=0}^{m} a_i C_i(s) + k\delta\alpha + k\delta\sum_{i=0}^{m} a_i A_i (s) + kr\delta\delta + r\delta\beta + r\delta\sum_{i=0}^{m} a_i B_i (s) + H(s)Z(s)$
\\
\\
\\ \texthl{$\alpha\beta$} $ + $ \texthl{$\alpha(\sum_{i=0}^{m} a_i B_i (s))$} $ + $ \texthl{$k\alpha\delta$} $ + $ \texthl{$\beta(\sum_{i=0}^{m} a_i A_i (s))$} $+ (\sum_{i=0}^{m} a_i A_i (s))(\sum_{i=0}^{m} a_i B_i (s)) + $ \texthl{$k\delta(\sum_{i=0}^{m} a_i A_i (s))$} $+ $ \texthl{$r\delta\beta$} $ + $ \texthl{$r\delta(\sum_{i=0}^{m} a_i B_i (s)$} $+ $ \texthl{$rk\delta\delta$} \textbf{\large=} \texthl{$\alpha\beta$} $ + $ \texthl{$\beta\sum_{i=0}^{m} a_i A_i (s)$} $ + $ \texthl{$\alpha\sum_{i=0}^{m} a_i B_i(s)$} $ + \sum_{i=0}^{m} a_i C_i(s) + $ \texthl{$k\delta\alpha$} $ + $\texthl{$k\delta\sum_{i=0}^{m} a_i A_i(s)$} $ + $ \texthl{$kr\delta\delta$} $+ $\texthl{$r\delta\beta$}$ + $\texthl{$r\delta\sum_{i=0}^{m} a_i B_i(s)$} $ + H(s)Z(s)$
\\
\\ $\Leftrightarrow (\sum_{i=0}^{m} a_i A_i (s))(\sum_{i=0}^{m} a_i B_i (s))$ \textbf{\large=} $\sum_{i=0}^{m} a_i C_i(s) + H(s)Z(s)$