\subsubsection{Prove function}
\underline{$Prove(R, \sigma, a_{i...l}, a_{l+1...m})$ :}
\tabNormal r$\xleftarrow[]{\$}$F
\tabNormal k$\xleftarrow[]{\$}$F
\tabNormal U = $\alpha + \sum_{i=0}^{m} a_i A_i (s) + r\delta $
\tabNormal V = $\beta + \sum_{i=0}^{m} a_i B_i (s) + k\delta $
\tabNormal We compute H(s) such that  \[ (\sum_{i=0}^m a_i A_i(s)) (\sum_{i=0}^m a_i B_i(s)) = \sum_{i=0}^m a_i C_i(s) + H(s) Z(s) \]
\tabNormal $\Aa =\sum_{i=l+1}^m a_i A_i$
\tabNormal $\Ba=\sum_{i=l+1}^m a_i B_i$
\tabNormal $\Ca =\sum_{i=l+1}^m a_i C_i$
\tabNormal $S=\frac{\beta \Aa (s) + \alpha \Ba (s) + \Ca (s)}{\delta}$
\tabNormal W = $S + \frac{H(s)Z(s)}{\delta} + Uk + rV - rk\delta $
\tabNormal $\pi = (U,V,W)$ 
\tabNormal return $\pi$